theories/L6_PCPS/Heap/cc_log_rel.v
@@ -7,7 +7,7 @@ From Coq Require Import NArith.BinNat Relations.Relations MSets.MSets
                         MSets.MSetRBT Lists.List omega.Omega Sets.Ensembles.
 From L6 Require Import functions cps eval cps_util identifiers ctx Ensembles_util
                        List_util Heap.heap Heap.heap_defs Heap.space_sem.
-From Libraries Require Import Coqlib.
+Require Import compcert.lib.Coqlib.
 
 Import ListNotations.
 
