theories/L6_PCPS/Heap/space_sem.v
@@ -8,7 +8,7 @@ From Coq Require Import NArith.BinNat Relations.Relations MSets.MSets
 From ExtLib Require Import Structures.Monad Data.Monads.OptionMonad Core.Type.
 From L6 Require Import cps cps_util eval List_util Ensembles_util functions
         identifiers Heap.heap Heap.heap_defs.
-From Libraries Require Import Coqlib.
+Require Import compcert.lib.Coqlib.
 
 Module SpaceSem (H : Heap).
 
