theories/L6_PCPS/closure_conversion_util.v
@@ -4,7 +4,7 @@
 
 From L6 Require Import cps size_cps cps_util set_util hoisting identifiers ctx
                        Ensembles_util List_util functions closure_conversion eval.
-Require Import Libraries.Coqlib.
+Require Import compcert.lib.Coqlib.
 Require Import Coq.ZArith.Znumtheory ArithRing Coq.Relations.Relations Coq.Arith.Wf_nat.
 Require Import Coq.Lists.List Coq.MSets.MSets Coq.MSets.MSetRBT Coq.Numbers.BinNums
         Coq.NArith.BinNat Coq.PArith.BinPos Coq.Sets.Ensembles Omega.
