theories/L6_PCPS/lambda_lifting_correct.v
@@ -5,7 +5,7 @@
 Require Import L6.cps L6.cps_util L6.set_util L6.hoisting L6.identifiers L6.ctx
         L6.Ensembles_util L6.alpha_conv L6.List_util L6.functions L6.lambda_lifting
         L6.eval L6.logical_relations L6.hoare.
-Require Import Libraries.Coqlib.
+Require Import compcert.lib.Coqlib.
 Require Import Coq.Lists.List Coq.MSets.MSets Coq.MSets.MSetRBT Coq.Numbers.BinNums
         Coq.NArith.BinNat Coq.PArith.BinPos Coq.Sets.Ensembles Omega.
 Require Import ExtLib.Structures.Monads ExtLib.Data.Monads.StateMonad.
